STLC_SuccNat/Lifted_Notations.v
@@ -3,7 +3,7 @@ Import ListNotations.
 Require Import Presence_Conditions_Notations.
 
 Declare Custom Entry ty'.
-Notation "<{{ e }}>'" := e (e custom ty' at level 99).
+Notation "'<{{ e }}>'" := e (e custom ty' at level 99).
 Notation "T" := T (in custom ty' at level 0, T constr at level 0).
 Notation "( T )" := T (in custom ty' at level 0, T custom ty' at level 99).
 Notation "T1 -> T2" := (Arrow' T1 T2)
@@ -12,15 +12,15 @@ Notation "T1 -> T2" := (Arrow' T1 T2)
 Notation "'Nat''" := Nat' (in custom ty' at level 0).
 Notation "'NatList''" := NatList' (in custom ty' at level 0).
 
-Check <{{ Nat' }}>'. (* Nat' : ty' *)
-Check <{{ NatList' }}>'. (* NatList' : ty' *)
-Check <{{ Nat' -> Nat' }}>'. (* Arrow' Nat' Nat' : ty' *)
-Check <{{ Nat' -> Nat' -> NatList' }}>'. (* Arrow' Nat' (Arrow' Nat' NatList') : ty' *)
-Check <{{ (Nat' -> Nat') -> NatList' }}>'. (* Arrow' (Arrow' Nat' Nat') NatList' : ty' *)
+Check '<{{ Nat' }}>'. (* Nat' : ty' *)
+Check '<{{ NatList' }}>'. (* NatList' : ty' *)
+Check '<{{ Nat' -> Nat' }}>'. (* Arrow' Nat' Nat' : ty' *)
+Check '<{{ Nat' -> Nat' -> NatList' }}>'. (* Arrow' Nat' (Arrow' Nat' NatList') : ty' *)
+Check '<{{ (Nat' -> Nat') -> NatList' }}>'. (* Arrow' (Arrow' Nat' Nat') NatList' : ty' *)
 
 Declare Custom Entry tm'.
 
-Notation "<{ e }>'" := e (e custom tm' at level 99).
+Notation "'<{ e }>'" := e (e custom tm' at level 99).
 
 Notation "( e )" := e
   (in custom tm' at level 0, e custom tm' at level 99).
@@ -35,22 +35,22 @@ Coercion var' : string >-> tm'.
 Notation "' x" := (var' x)
   (in custom tm' at level 1, x constr at level 0).
 
-Check <{ [(42,<[T]>)] }>'.       (* const' [(42,pc_True)] : tm' *)
-Check <{ '"f" }>'.     (* var "f" : tm' *)
-Check <{ ('"f") }>'.   (* var "f" : tm' — constr escape still works *)
-Check <{ ([(42,<[T]>)]) }>'.     (* const 42 : tm' — constr escape still works *)
+Check '<{ [(42,<[T]>)] }>'.       (* const' [(42,pc_True)] : tm' *)
+Check '<{ '"f" }>'.     (* var "f" : tm' *)
+Check '<{ ('"f") }>'.   (* var "f" : tm' — constr escape still works *)
+Check '<{ ([(42,<[T]>)]) }>'.     (* const 42 : tm' — constr escape still works *)
 
 Notation "t1 t2" := (app' t1 t2)
   (in custom tm' at level 20, left associativity,
    t1 custom tm', t2 custom tm' at level 19).
 
-Check <{ '"f" '"x" }>'.
+Check '<{ '"f" '"x" }>'.
 (* app' (var' "f") (var' "x") : tm' *)
-Check <{ '"f" '"x" '"y" }>'.
+Check '<{ '"f" '"x" '"y" }>'.
 (* app' (app' (var' "f") (var' "x")) (var' "y") : tm' *)
-Check <{ '"f" ('"x" '"y") }>'.
+Check '<{ '"f" ('"x" '"y") }>'.
 (* app' (var' "f") (app' (var' "x") (var' "y")) : tm' *)
-Check <{ '"f" [(42,<["A"]>)] }>'.
+Check '<{ '"f" [(42,<["A"]>)] }>'.
 (* app' (var' "f") (const'[(42,"A")] ) : tm' *)
 
 Notation "\ x : T , t" := (abs' x T t)
@@ -59,47 +59,47 @@ Notation "\ x : T , t" := (abs' x T t)
    T custom ty' at level 99,
    t custom tm' at level 99).
 
-Check <{ \"f" : Nat' , '"f" }>'. 
+Check '<{ \"f" : Nat' , '"f" }>'. 
 (* abs' "f" Nat' (var' "f") : tm' *)
 
-Check <{ \"f" : Nat' -> Nat' , '"f" [(42, <[~"A"]>)] }>'.
+Check '<{ \"f" : Nat' -> Nat' , '"f" [(42, <[~"A"]>)] }>'.
 (* abs' "f" (Arrow' Nat' Nat') (app' (var' "f") (const' 42)) : tm' *)
 
-Check <{ \"f" : Nat' , \"x" : Nat' , '"f" '"x" }>'.
+Check '<{ \"f" : Nat' , \"x" : Nat' , '"f" '"x" }>'.
 (* abs' "f" Nat' (abs' "x" Nat' (app' (var' "f") (var' "x"))) : tm' *)
 
-Check <{ (\"f" : Nat' , '"f") [(42, <[~"A"]>)] }>'.
+Check '<{ (\"f" : Nat' , '"f") [(42, <[~"A"]>)] }>'.
 (* app' (abs' "f" Nat' (var' "f")) (const' [(42,~"A")]) : tm' *)
 
-Notation "'succ'' t" := (succ' t)
+Notation "'s' t" := (succ' t)
   (in custom tm' at level 89,
    t custom tm' at level 89).
 
-Check <{ succ' [(42,<["A"]>)] }>'.
+Check '<{ s [(42,<["A"]>)] }>'.
 (* succ' (const' [(42,<["A"]>)]) : tm' *)
-Check <{ succ' '"f" }>'.
+Check '<{ s '"f" }>'.
 (* succ' (var' "f") : tm' *)
-Check <{ succ' succ' [(42,<["A"]>)] }>'.
+Check '<{ s s [(42,<["A"]>)] }>'.
 (* succ' (succ' (const' 42)) : tm' *)
-Check <{ (\"f" : Nat' , succ' '"f") [(42,<["A"]>)] }>'.
+Check '<{ (\"f" : Nat' , s '"f") [(42,<["A"]>)] }>'.
 (* app' (abs' "f" Nat' (succ' (var' "f"))) (const' [(42,<["A"]>)]) : tm' *)
 
 Notation "t1 + t2" := (add' t1 t2)
   (in custom tm' at level 50, left associativity,
    t1 custom tm', t2 custom tm' at level 49).
 
-Check <{ [(42,<[T]>)] + [(1,<[T]>)] }>'.                     (* add (const 42) (const 1) : tm' *)
-Check <{ succ' [(1,<[T]>)] + [(2,<[T]>)] }>'.              (* add (succ (const 1)) (const 2) : tm' *)
+Check '<{ [(42,<[T]>)] + [(1,<[T]>)] }>'.                     (* add (const 42) (const 1) : tm' *)
+Check '<{ s [(1,<[T]>)] + [(2,<[T]>)] }>'.              (* add (succ (const 1)) (const 2) : tm' *)
 
-Notation "'nil''" := nil' (in custom tm' at level 0).
+Notation "'nil'" := nil' (in custom tm' at level 0).
 
 Notation "t1 :: t2" := (cons' t1 t2)
   (in custom tm' at level 60, right associativity,
    t1 custom tm', t2 custom tm' at level 60).
 
-Check <{ nil' }>'.
+Check '<{ nil }>'.
 (* nil' : tm' *)
-Check <{ ([(1,<[T]>)] :: [(2,<[F]>)] :: nil') }>'.
+Check '<{ ([(1,<[T]>)] :: [(2,<[F]>)] :: nil) }>'.
 (*Removed because creates conflicts with variational values notations. *)
 (*Notation "[ t ]" := (cons' t nil')
   (in custom tm' at level 0, t custom tm' at level 60).
@@ -114,19 +114,19 @@ Check <{ [1 ; 2] }>.     (* cons (const 1) (cons (const 2) nil) : tm' *)
 Check <{ [1 ; 2 ; 3] }>. (* cons (const 1) (cons (const 2) (cons (const 3) nil)) : tm' *)
  *)
 
-Notation "'case' t1 'of' '|' 'nil'' '=>' t2 '|' h :: t '=>' t3" := (case' t1 t2 h t t3)
+Notation "'case' t1 'of' '|' 'nil' '=>' t2 '|' h :: t '=>' t3" := (case' t1 t2 h t t3)
   (in custom tm' at level 89,
    t1 custom tm' at level 99,
    t2 custom tm' at level 99,
    h constr at level 0,
    t constr at level 0,
    t3 custom tm' at level 99,
-   format "'[hv' 'case'  t1  'of' '//' '|'  'nil''  '=>'  t2 '//' '|'  h  '::'  t  '=>'  t3 ']'").
+   format "'[hv' 'case'  t1  'of' '//' '|'  'nil'  '=>'  t2 '//' '|'  h  '::'  t  '=>'  t3 ']'").
 
-Check <{ case nil' of | nil' => [(0,<[T]>)] | "h" :: "t" => succ' '"h" }>'.
+Check '<{ case nil of | nil => [(0,<[T]>)] | "h" :: "t" => s '"h" }>'.
 
-Check <{ case ([(1,<[T]>)] :: [(2,<[F]>)] :: nil') of
-          | nil' => [(0,<[T]>)]
+Check '<{ case ([(1,<[T]>)] :: [(2,<[F]>)] :: nil) of
+          | nil => [(0,<[T]>)]
           | "h" :: "t" => '"h" + '"t" }>'.
 (* case (cons (const 1) (cons (const 2) nil)) (const 0) "h" "t" (add (var "h") (var "t")) : tm' *)
 
